theories/GeneralizeLtsOutputs.v
@@ -34,166 +34,7 @@ Require Import Coq.Program.Equality.
 From Coq.Logic Require Import ProofIrrelevance.
 
 From stdpp Require Import base countable list decidable finite gmap gmultiset.
-From Must Require Import TransitionSystems.
-
-(** Actions  *)
-
-Inductive ExtAct (A: Type) :=
-| ActIn (a : A)
-| ActOut (a : A)
-.
-Arguments ActIn {_} _.
-Arguments ActOut {_} _.
-
-Definition ext_act_match {A} (l1 l2: ExtAct A) :=
-  match l1, l2 with
-  | ActIn x, ActOut y => x = y
-  | ActOut x, ActIn y => x = y
-  | _, _ => False
-  end.
-
-Inductive Act (A: Type) :=
-| ActExt (μ: ExtAct A)
-| τ
-.
-Arguments ActExt {_} _.
-Arguments τ {_}.
-
-Definition co {A} (l: ExtAct A) :=
-  match l with
-  | ActIn x => ActOut x
-  | ActOut x => ActIn x
-  end.
-
-Lemma co_involution {A} (l: ExtAct A) : co (co l) = l.
-Proof. destruct l; eauto. Qed.
-
-Definition ext_match_commutative {A} (l1 l2: ExtAct A):
-  ext_act_match l1 l2 -> ext_act_match l2 l1.
-Proof. by destruct l1 as [?|?], l2 as [?|?]; eauto; intros ->. Qed.
-
-#[global] Instance actext_eqdec `{EqDecision L} : EqDecision (ExtAct L).
-Proof. solve_decision. Defined.
-#[global] Instance act_eqdec `{EqDecision L} : EqDecision (Act L).
-Proof. solve_decision. Defined.
-#[global] Instance ext_act_match_dec `{EqDecision L} : ∀ (ℓ1 ℓ2: ExtAct L), Decision (ext_act_match ℓ1 ℓ2).
-Proof.
-  intros [l1|l1] [l2|l2]; [by right; intros ? | | | by right; intros ?];
-    destruct (decide (l1 = l2)); eauto.
-Defined.
-
-Definition trace L := list (ExtAct L).
-
-Definition is_input {A} (μ : ExtAct A) := ∃ a, μ = ActIn a.
-
-Definition are_inputs {A} (s : trace A) := Forall is_input s.
-
-Definition is_output {A} (μ : ExtAct A) := ∃ a, μ = ActOut a.
-
-Definition are_outputs {A} (s : trace A) := Forall is_output s.
-
-
-Class Label (L: Type) :=
-  MkLabel {
-      label_eqdec: EqDecision L;
-      label_countable: Countable L;
-    }.
-#[global] Existing Instance label_eqdec.
-#[global] Existing Instance label_countable.
-
-Class Lts (A L : Type) `{Label L} :=
-  MkLts {
-      lts_step: A → Act L → A → Prop;
-      lts_state_eqdec: EqDecision A;
-
-      lts_step_decidable a α b : Decision (lts_step a α b);
-
-      lts_outputs : A -> gset L;
-      lts_outputs_spec1 p1 x p2 : lts_step p1 (ActExt (ActOut x)) p2 -> x ∈ lts_outputs p1;
-      lts_outputs_spec2 p1 x : x ∈ lts_outputs p1 -> {p2 | lts_step p1 (ActExt (ActOut x)) p2};
-
-      lts_stable: A → Act L → Prop;
-      lts_stable_decidable p α : Decision (lts_stable p α);
-      lts_stable_spec1 p α : ¬ lts_stable p α → { q | lts_step p α q };
-      lts_stable_spec2 p α : { q | lts_step p α q } → ¬ lts_stable p α;
-    }.
-#[global] Existing Instance lts_state_eqdec.
-#[global] Existing Instance lts_step_decidable.
-#[global] Existing Instance lts_stable_decidable.
-
-Notation "p ⟶ q"      := (lts_step p τ q) (at level 30, format "p  ⟶  q").
-Notation "p ⟶{ α } q" := (lts_step p α q) (at level 30, format "p  ⟶{ α }  q").
-Notation "p ⟶[ μ ] q" := (lts_step p (ActExt μ) q) (at level 30, format "p  ⟶[ μ ]  q").
-
-Notation "p ↛"      := (lts_stable p τ) (at level 30, format "p  ↛").
-Notation "p ↛{ α }" := (lts_stable p α) (at level 30, format "p  ↛{ α }").
-Notation "p ↛[ μ ]" := (lts_stable p (ActExt μ)) (at level 30, format "p  ↛[ μ ]").
-
-Class FiniteLts A L `{Lts A L} :=
-  MkFlts {
-      folts_states_countable: Countable A;
-      folts_next_states_finite p α : Finite (dsig (fun q => lts_step p α q));
-}.
-
-#[global] Existing Instance folts_states_countable.
-#[global] Existing Instance folts_next_states_finite.
-
-Class LtsEq (A L : Type) `{Lts A L} := {
-    (* todo: use Equivalence *)
-    eq_rel : A -> A -> Prop;
-    eq_rel_refl p : eq_rel p p;
-    eq_symm p q : eq_rel p q -> eq_rel q p;
-    eq_trans p q r : eq_rel p q -> eq_rel q r -> eq_rel p r;
-    (* reference: L 1.4.15 p.51 Sangiorgi pi-book *)
-    eq_spec p q (α : Act L) : (exists r, eq_rel p r /\ r ⟶{α} q) -> (exists r, p ⟶{α} r /\ eq_rel r q);
-  }.
-
-Add Parametric Relation `{Lts A L, ! LtsEq A L} : A eq_rel
-    reflexivity proved by (eq_rel_refl)
-    symmetry proved by (eq_symm)
-    transitivity proved by (eq_trans)
-    as sc_proc_rel.
-
-Infix "⋍" := eq_rel (at level 70).
-
-Definition lts_sc `{Lts A L, !LtsEq A L} p α q := exists r, p ⟶{α} r /\ r ⋍ q.
-
-Notation "p ⟶⋍ q" := (lts_sc p τ q) (at level 30, format "p  ⟶⋍  q").
-Notation "p ⟶⋍{ α } q" := (lts_sc p α q) (at level 30, format "p  ⟶⋍{ α }  q").
-Notation "p ⟶⋍[ μ ] q" := (lts_sc p (ActExt μ) q) (at level 30, format "p  ⟶⋍[ μ ]  q").
-
-Class LtsOba (A L : Type) `{Lts A L, !LtsEq A L} :=
-  MkOBA {
-      (* Multiset of outputs *)
-      lts_oba_mo p : gmultiset L;
-      lts_oba_mo_spec1 p a : a ∈ lts_oba_mo p <-> a ∈ lts_outputs p;
-      lts_oba_mo_spec2 p a : forall q, p ⟶[ActOut a] q -> lts_oba_mo p = {[+ a +]} ⊎ lts_oba_mo q;
-      (* Selinger axioms. *)
-      lts_oba_output_commutativity {p q r a α} :
-      p ⟶[ActOut a] q -> q ⟶{α} r -> (∃ t, p ⟶{α} t /\ t ⟶⋍[ActOut a] r) ;
-      lts_oba_output_confluence {p q1 q2 a μ} :
-      μ ≠ ActOut a -> p ⟶[ActOut a] q1 -> p ⟶[μ] q2 ->
-      ∃ r, q1 ⟶[μ] r /\ q2 ⟶⋍[ActOut a] r ;
-      lts_oba_output_tau {p q1 q2 a} :
-      p ⟶[ActOut a] q1 -> p ⟶ q2 -> (∃ t, q1 ⟶ t /\ q2 ⟶⋍[ActOut a] t) \/ q1 ⟶⋍[ActIn a] q2 ;
-      lts_oba_output_deter {p1 p2 p3 a} :
-      p1 ⟶[ActOut a] p2 -> p1 ⟶[ActOut a] p3 -> p2 ⋍ p3 ;
-      (* Extra axiom, it would be nice to remove it, not used that much. *)
-      lts_oba_output_deter_inv {p1 p2 q1 q2} a :
-      p1 ⟶[ActOut a] q1 -> p2 ⟶[ActOut a] q2 -> q1 ⋍ q2 -> p1 ⋍ p2
-    }.
-
-Class LtsObaFB (A L: Type) `{LtsOba A L} :=
-  MkLtsObaFB {
-      lts_oba_fb_feedback {p1 p2 p3 a} : p1 ⟶[ActOut a] p2 -> p2 ⟶[ActIn a] p3 -> p1 ⟶⋍ p3
-    }.
-
-Class LtsObaFW (A L : Type) `{LtsOba A L} :=
-  MkLtsObaFW {
-      lts_oba_fw_forward p1 a : ∃ p2, p1 ⟶[ActIn a] p2 /\ p2 ⟶[ActOut a] p1 ;
-      lts_oba_fw_feedback {p1 p2 p3 a} : p1 ⟶[ActOut a] p2 -> p2 ⟶[ActIn a] p3 -> p1 ⟶⋍ p3 \/ p1 ⋍ p3 ;
-    }.
-
+From Must Require Import TransitionSystems OldTransitionSystems.
 
 (* Genarilization via essential actions, non_blocking actions *)
 
@@ -222,11 +63,33 @@ Proof.
   + intro. subst. simpl. eauto.
 Qed.
 
+Definition encode_ext_act `{Label A} (μ : ExtAct A) : gen_tree (A + A) :=
+match μ with
+  | ActIn a => GenLeaf (inr a)
+  | ActOut a => GenLeaf (inl a)
+end.
+
+Definition decode_ext_act `{Label A} (tree : gen_tree (A + A)) : option (ExtAct A) :=
+match tree with
+  | GenLeaf (inr a) => Some (ActIn a)
+  | GenLeaf (inl a) => Some (ActOut a)
+  | _ => None
+end.
+
+Lemma encode_decide_ext_act `{Label A} μ : decode_ext_act (encode_ext_act μ) = Some μ.
+Proof. case μ. 
+* intros. simpl. reflexivity.
+* intros. simpl. reflexivity.
+Qed.
+
+
+#[global] Instance ext_act_countable `{Label A} : Countable (ExtAct A).
+Proof.
+  refine (inj_countable encode_ext_act decode_ext_act encode_decide_ext_act).
+Qed.
+
 #[global] Program Instance gLabel
   `{Label A} : TransitionSystems.ExtAction (ExtAct A).
-Next Obligation.
-  intros. admit.
-Admitted.
 Next Obligation.
   intros L H μ. exact (is_output μ).
 Defined.
@@ -242,7 +105,12 @@ Next Obligation.
   intros. unfold relation. exact ext_act_match.
 Defined.
 Next Obligation.
-  intros. unfold sc. unfold gLabel_obligation_5.
+  intros. exists (co η). unfold sc. 
+  unfold gLabel_obligation_4. unfold ext_act_match.
+  destruct η; simpl in *; eauto. 
+Defined.
+Next Obligation.
+  intros. unfold sc. unfold gLabel_obligation_4.
   destruct a; destruct b.
   + right. intro cases. eauto. destruct cases as [case_1 | case_2].
     ++ eapply simplify_match_input in case_1. inversion case_1.
@@ -262,14 +130,35 @@ Next Obligation.
   + simpl in *. right. intro Hyp. destruct Hyp; eauto.
 Defined.
 Next Obligation.
-  intros. exists (co η). unfold sc. 
-  unfold gLabel_obligation_5. unfold ext_act_match.
-  destruct η; simpl in *; eauto. 
+  unfold gLabel_obligation_1.
+  unfold gLabel_obligation_4.
+  intros A H η μ IsOut eq.
+  intro IsOut'. destruct IsOut' as (μ' & eq'); subst.
+  unfold sc in eq.
+  destruct eq as [eq_1 | eq_2].
+  + symmetry in eq_1.
+    eapply simplify_match_output in eq_1. subst.
+    destruct IsOut as ( a & impossible).
+    inversion impossible.
+  + eapply simplify_match_output in eq_2. subst.
+    destruct IsOut as ( a & impossible).
+    inversion impossible.
+Defined.
+Next Obligation.
+  unfold gLabel_obligation_1.
+  unfold gLabel_obligation_4.
+  unfold sc. unfold gLabel_obligation_3.
+  intros A H η μ IsOut eq.
+  destruct IsOut as (η' & eq'); subst.
+  destruct eq as [eq_1 | eq_2].
+  + eapply simplify_match_output in eq_1. subst. simpl. eauto.
+  + symmetry in eq_2.
+    eapply simplify_match_output in eq_2. subst. simpl. eauto.
 Defined.
 Next Obligation. 
-  unfold sc. unfold gLabel_obligation_2.
-  unfold gLabel_obligation_5.
-  intros ? ? ? ? ? (a & eq) Hyp Hyp'. subst.
+  unfold sc. unfold gLabel_obligation_1.
+  unfold gLabel_obligation_4.
+  intros A ? ? ? ? (a & eq) Hyp Hyp'. subst.
   destruct Hyp as [case_1 | case_2]; destruct Hyp' as [case_1' | case_2']; exists a; eauto.
   + eapply simplify_match_output in case_1. subst.
     symmetry in case_1'. eapply simplify_match_input in case_1'. subst.
@@ -283,40 +172,283 @@ Next Obligation.
     eapply simplify_match_output in case_2. subst.
     eapply simplify_match_input in case_2'. subst.
     eauto.
-Qed.
-Next Obligation.
-  unfold gLabel_obligation_2.
-  unfold gLabel_obligation_5.
-  intros A H η μ IsOut eq.
-  intro IsOut'. destruct IsOut' as (μ' & eq'); subst.
-  unfold sc in eq.
-  destruct eq as [eq_1 | eq_2].
-  + symmetry in eq_1.
-    eapply simplify_match_output in eq_1. subst.
-    destruct IsOut as ( a & impossible).
-    inversion impossible.
-  + eapply simplify_match_output in eq_2. subst.
-    destruct IsOut as ( a & impossible).
-    inversion impossible.
-Qed.
-Next Obligation.
-  unfold gLabel_obligation_2.
-  unfold gLabel_obligation_5.
-  unfold sc. unfold gLabel_obligation_4.
-  intros A H η μ IsOut eq.
-  destruct IsOut as (η' & eq'); subst.
-  destruct eq as [eq_1 | eq_2].
-  + eapply simplify_match_output in eq_1. subst. simpl. eauto.
-  + symmetry in eq_2.
-    eapply simplify_match_output in eq_2. subst. simpl. eauto.
-Qed.
+Defined.
 
 
 #[global] Program Instance gLts
-  `{LtsP: Lts P A} : TransitionSystems.Lts P A :=
-  {|
-    lts_step := lts_step;
-  |}.
+  `{LtsP: Lts P A} : gLts P (ExtAct A).
+Next Obligation.
+  intros ? ? ? ? p1 α p2.
+  destruct α as [|].
+  + exact (lts_step p1 (ActExt μ) p2).
+  + exact (lts_step p1 τ p2).
+Defined.
+Next Obligation.
+  intros ? ? ? ? p1 α p2. unfold gLts_obligation_1.
+  destruct α as [ μ |].
+  + exact (lts_step_decidable p1 (ActExt μ) p2).
+  + exact (lts_step_decidable p1 τ p2).
+Defined.
+Next Obligation.
+  intros ? ? ? LtsP p α. 
+  destruct α as [ μ |].
+  + exact (lts_stable p (ActExt μ)).
+  + exact (lts_stable p τ).
+Defined.
+Next Obligation.
+  unfold gLts_obligation_3.
+  destruct α as [ μ |].
+  + exact (lts_stable_decidable p (ActExt μ)).
+  + exact (lts_stable_decidable p τ).
+Defined.
+Next Obligation.
+  unfold gLts_obligation_3.
+  destruct α as [ μ |].
+  + intro not_stable. exact (lts_stable_spec1 p (ActExt μ) not_stable).
+  + intro not_stable. exact (lts_stable_spec1 p τ not_stable).
+Qed.
+Next Obligation.
+  unfold gLts_obligation_1.
+  unfold gLts_obligation_3.
+  destruct α as [ μ |].
+  + intro wit_not_stable. exact (lts_stable_spec2 p (ActExt μ) wit_not_stable).
+  + intro wit_not_stable. exact (lts_stable_spec2 p τ wit_not_stable).
+Defined.
+
+
+#[global] Program Instance gFiniteLts
+  `{FiniteLts P A} : FiniteImagegLts P (ExtAct A).
+Next Obligation.
+  intros.
+  destruct α as [ μ |].
+  + exact (folts_next_states_finite p (ActExt μ)).
+  + exact (folts_next_states_finite p τ).
+Defined.
+
+#[global] Program Instance gLtsEq
+  `{LtsEq P A} : gLtsEq P (ExtAct A).
+Next Obligation.
+  intros ? ? ? LtsP LtsEqP p q α Hyp. 
+  destruct α as [ μ |].
+  + exact (eq_spec p q (ActExt μ) Hyp).
+  + exact (eq_spec p q τ Hyp).
+Defined.
+
+Definition label_to_output `{Label A} (a : A) : ExtAct A := ActOut a.
+
+Definition mo_label_to_mo_output `{Label A} (m : gmultiset A) : gmultiset (ExtAct A) :=
+    gmultiset_map label_to_output m.
+
+Definition set_label_to_mo_output `{Label A} (m : gset A) : gset (ExtAct A) :=
+    list_to_set (fmap label_to_output (elements m)).
+
+(* #[global] Instance output_in_gmultiset_dec `{Prop_of_Inter S1 S2 A} 
+  η x p1 :
+  Decision (η = label_to_output x ∧ x ∈ lts_oba_mo p1). *)
+
+
+#[global] Program Instance gLtsOba
+  `{LtsOba P A} : gLtsOba P (ExtAct A).
+Next Obligation.
+  intros.
+  exact (mo_label_to_mo_output (lts_oba_mo p)).
+Defined.
+Next Obligation.
+  intros ? ? ? ? ? ? ? ? ? nb l. unfold gLtsOba_obligation_1.
+  destruct η as [a | a].
+  + exfalso. inversion nb. inversion H2.
+  + eapply elem_of_gmultiset_map.
+    exists a. split.
+      ++ unfold label_to_output. eauto.
+      ++ eapply lts_oba_mo_spec1.
+         eapply lts_outputs_spec1.
+         exact l.
+Defined.
+Next Obligation.
+  unfold gLtsOba_obligation_1.
+  intros ? ? ? ? ? ? ? ? Hyp. 
+  eapply elem_of_gmultiset_map in Hyp.
+  
+  assert ({ x : A | η = label_to_output x ∧ x ∈ lts_oba_mo p1}) as (a & eq & mem).
+  eapply choice; eauto. intros.
+  destruct (decide (η = label_to_output x)) as [eq | not_eq].
+  + destruct (decide (x ∈ lts_oba_mo p1)).
+    ++ left. split; eauto.
+    ++ right. intro Hyp'. destruct Hyp' as (eq' & imp). contradiction.
+  + right. intro Hyp'. destruct Hyp' as (eq' & imp). contradiction.
+  
+  + eapply lts_oba_mo_spec1 in mem.
+    eapply lts_outputs_spec2 in mem as (q & l).
+    exists q. split.
+    ++ exists a. subst. eauto.
+    ++ rewrite eq. unfold label_to_output. exact l.
+Qed.
+Next Obligation.
+  unfold gLtsOba_obligation_1.
+  intros ? ? ? ? ? LtsOBAP ? ? ? nb Hyp;simpl in *.
+  destruct nb as (a & eq). subst.
+  assert (lts_oba_mo p = {[+ a +]} ⊎ lts_oba_mo q) as mem.
+  eapply lts_oba_mo_spec2. exact Hyp.
+  rewrite mem. simpl in *. unfold mo_label_to_mo_output at 1.
+  rewrite gmultiset_map_disj_union. rewrite gmultiset_map_singleton.
+  unfold label_to_output at 1. reflexivity.
+Qed.
+Next Obligation. (* lts_oba_non_blocking_action_delay *)
+  intros ? ? ? ? ? LtsOBAP ? ? ? ? ? nb l1 l2 ;simpl in *.
+  unfold gLts_obligation_1 in l2.
+  destruct nb as (a & eq); subst. 
+  destruct α as [|].
+  + destruct μ as [a' | a'].
+    ++ eapply lts_oba_output_commutativity; eauto.
+    ++ eapply lts_oba_output_commutativity; eauto.
+  + eapply lts_oba_output_commutativity; eauto. 
+Qed.
+Next Obligation. (* lts_oba_non_blocking_action_confluence *)
+  intros ? ? ? ? ? LtsOBAP ? ? ? ? ? nb eq l1 l2 ;simpl in *.
+  destruct nb as (a & eq'); subst.
+  eapply lts_oba_output_confluence; eauto.
+Qed.
+Next Obligation. (* lts_oba_output_tau *)
+  intros ? ? ? ? ? LtsOBAP ? ? ? ? nb l1 l2 ;simpl in *.
+  destruct nb as (a & eq); subst.
+  unfold gLabel_obligation_4.
+  eapply lts_oba_output_tau in l1 as cases; eauto.
+  destruct cases as [computation_without_a | computation_with_a].
+  + left. destruct computation_without_a as (t & l'1 & l'2).
+    exists t; eauto.
+  + right. exists (ActIn a). split; eauto.
+    unfold sc. simpl. eauto.
+Qed.
+Next Obligation. (* lts_oba_output_deter *)
+  intros ? ? ? ? ? LtsOBAP ? ? ? ? nb l1 l2 ;simpl in *.
+  destruct nb as (a & eq); subst. 
+  eapply lts_oba_output_deter; eauto.
+Qed.
+Next Obligation. (* lts_oba_non_blocking_action_deter_inv *)
+  intros ? ? ? ? ? LtsOBAP ? ? ? ? ? nb l1 l2 ;simpl in *.
+  destruct nb as (a & eq); subst.
+  eapply lts_oba_output_deter_inv; eauto.
+Qed.
+
+#[global] Program Instance gLtsObaFB
+  `{LtsObaFB P A} : gLtsObaFB P (ExtAct A).
+Next Obligation.
+  intros ? ? ? ? ? LtsOBAP ? ? ? ? ? ? nb duo l1 l2 ;simpl in *.
+  destruct nb as (a & eq); subst.
+  destruct duo as [case_1 | case_2].
+  + eapply simplify_match_output in case_1; subst.
+    eapply lts_oba_fb_feedback; eauto.
+  + symmetry in case_2.
+    eapply simplify_match_output in case_2; subst.
+    eapply lts_oba_fb_feedback; eauto.
+Qed.
+
+#[global] Program Instance gLtsObaFW
+  `{LtsObaFW P A} : gLtsObaFW P (ExtAct A).
+Next Obligation.
+  intros ? ? ? ? ? ? ? p η μ ;simpl in *.
+  destruct (decide (non_blocking η)) as [nb | not_nb].
+  + destruct nb as (a & eq); subst.
+    unfold gLabel_obligation_1. unfold gLabel_obligation_4.
+    destruct (lts_oba_fw_forward p a) as (p' & l1 & l2).
+    exists p'. intros Hyp duo. destruct duo as [case_1 | case_2].
+    ++ eapply simplify_match_output in case_1; subst. split;eauto.
+    ++ eapply symmetry, simplify_match_output in case_2; subst. split;eauto.
+  + exists p. intro. contradiction.
+Qed.
+
+#[global] Program Instance Inter_FW
+  `{LtsP : Lts P A} : 
+    Prop_of_Inter P (TransitionSystems.mb (ExtAct A)) (ExtAct A) fw_inter.
+Next Obligation.
+  intros ? ? ? ? p. exact (set_label_to_mo_output (lts_outputs p)).
+Defined.
+Next Obligation.
+  unfold Inter_FW_obligation_1. unfold set_label_to_mo_output.
+  intros ? ? ? ? ? ? Hyp ;simpl in *.
+  eapply elem_of_list_to_set in Hyp.
+  eapply elem_of_list_fmap in Hyp.
+
+  assert {x : A | ξ = label_to_output x ∧ x ∈ elements (lts_outputs p)} as wit.
+  eapply choice;eauto. intro.
+  destruct (decide (ξ = label_to_output x)).
+  + destruct (decide (x ∈ elements (lts_outputs p))).
+    ++ left; eauto.
+    ++ right. intros (Hyp1 & imp). contradiction.
+  + right. intros (imp & Hyp2). contradiction.
+  
+  + destruct wit as ( a & eq & mem ).
+    unfold label_to_output in eq; subst.
+    assert (a ∈ lts_outputs p) as mem'.
+    eapply elem_of_elements; eauto.
+    eapply lts_outputs_spec2 in mem'. 
+    eauto.
+Qed.
+Next Obligation.
+  intros ? ? ? ? m;simpl in *.
+  exact (dom (mb_without_not_nb m)).
+Defined.
+Next Obligation.
+  unfold Inter_FW_obligation_3.
+  intros ? ? ? ? m ? Hyp ;simpl in *.
+  eapply gmultiset_elem_of_dom in Hyp. 
+  assert (ξ ∈ mb_without_not_nb m) as mem. eauto.
+  eapply lts_mb_nb_with_nb_spec1 in mem as (nb & eq).
+  eapply gmultiset_disj_union_difference' in eq.
+  exists (m ∖ {[+ ξ +]}). rewrite eq at 1.
+  eapply lts_multiset_minus; eauto.
+Defined.
+Next Obligation.
+  intros ? ? ? ? ? ? ? m ? m' ? ? inter;simpl in *.
+  right. destruct inter as (duo & nb).
+  unfold Inter_FW_obligation_3.
+  eapply gmultiset_elem_of_dom.
+  eapply non_blocking_action_in_ms in nb as eq'; eauto. 
+  rewrite<- eq'.
+  assert (mb_without_not_nb ({[+ α2 +]} ⊎ m') 
+  = {[+ α2 +]} ⊎ (mb_without_not_nb m')) as eq.
+  eapply lts_mb_nb_spec1; eauto. rewrite eq.
+  multiset_solver.
+Defined.
+Next Obligation.
+  intros ? ? ? ? ξ p;simpl in *.
+  destruct ξ as [ a (* Input_case *) | a (* Ouput_case *)].
+  + exact empty. 
+  + exact {[ ActIn a ]}.
+Defined.
+Next Obligation.
+  unfold Inter_FW_obligation_6.
+  unfold Inter_FW_obligation_3.
+  intros ? ? ? ? ? ? ? ? m mem l inter;simpl in *.
+  destruct inter as (duo & nb). destruct nb as (a & eq).
+  subst. destruct duo as [case_1 | case_2]; unfold gLabel_obligation_4 in *.
+  + eapply simplify_match_output in case_1. subst. set_solver.
+  + symmetry in case_2. eapply simplify_match_output in case_2. subst. set_solver.
+Defined.
+Next Obligation.
+  intros. exact empty.
+Defined.
+Next Obligation.
+  unfold Inter_FW_obligation_8. unfold Inter_FW_obligation_1.
+  intros ? ? ? ? ? ? ? ? m mem l inter;simpl in *.
+  exfalso.
+  destruct inter as (duo & nb). destruct nb as (a & eq). subst.
+  unfold set_label_to_mo_output in mem.
+  eapply elem_of_list_to_set in mem.
+  eapply elem_of_list_fmap in mem. destruct mem as (a' & eq & mem').
+  subst. destruct duo as [case_1 | case_2].
+  + eapply simplify_match_output in case_1. inversion case_1.
+  + eapply simplify_match_output in case_2. inversion case_2.
+Defined.
+
+
+#[global] Program Instance Inter_par
+  `{@Lts P A H} `{@Lts Q A H}: 
+    Prop_of_Inter P Q (ExtAct A) parallel_inter (* (@gLabel A H) gLts gLts *).
+Next Obligation.
+Admitted.
+Next Obligation.
+Admitted.
 Next Obligation.
 Admitted.
 Next Obligation.
@@ -332,7 +464,32 @@ Admitted.
 Next Obligation.
 Admitted.
 
+#[global] Program Instance Inter_FW_par
+  `{@Lts P A H} `{@Lts E A H}: Prop_of_Inter (P * mb A) E (ExtAct A) parallel_inter.
+Next Obligation.
+Admitted.
+Next Obligation.
+Admitted.
+Next Obligation.
+Admitted.
+Next Obligation.
+Admitted.
+Next Obligation.
+Admitted.
+Next Obligation.
+Admitted.
+Next Obligation.
+Admitted.
+Next Obligation.
+Admitted.
+Next Obligation.
+Admitted.
 
+Lemma com_only_with_non_blocking `{LtsP : Lts P A} (η : ExtAct A) η': 
+        dual η η' -> non_blocking η \/ non_blocking η'.
+Proof.
+Admitted.
 
+Lemma (p , m) 
 
 
